two admits remaining

theories/TM/L/CompilerBoolFuns/ClosedLAdmissible.v
@@ -4,8 +4,8 @@ From Undecidability.Shared.Libs.PSL Require Import Vectors.
 From Coq Require Import Vector List.
 
 From Undecidability.L Require Import L LTactics L_facts Functions.Eval Functions.Decoding Functions.Encoding.
-From Undecidability.L.Datatypes Require Import LBool Lists LVector.
-From Undecidability.L.Complexity.LinDecode Require Import LTDbool LTDlist.
+From Undecidability.L.Datatypes Require Import LBool Lists LVector List.List_fold.
+From Undecidability.L.Complexity.LinDecode Require Import LTDbool LTDlist LTDnat.
 
 From Undecidability.TM.L.CompilerBoolFuns Require Import Compiler_spec NaryApp.
 
@@ -13,6 +13,11 @@ From Undecidability.TM.L.CompilerBoolFuns Require Import Compiler_spec NaryApp.
 Import ListNotations.
 Import VectorNotations.
 Import L_Notations. 
+
+Definition L_computable_closed {k} (R : Vector.t nat k -> nat -> Prop) := 
+  exists s, closed s /\ forall v : Vector.t nat k, 
+      (forall m, R v m <-> L.eval (Vector.fold_left (fun s n => L.app s (encNatL n)) s v) (encNatL m)) /\
+      (forall o, L.eval (Vector.fold_left (fun s n => L.app s (encNatL n)) s v) o -> exists m, o = encNatL m).
 
 Definition L_bool_computable_closed {k} (R : Vector.t (list bool) k -> (list bool) -> Prop) := 
   exists s, closed s /\ forall v : Vector.t (list bool) k, 
@@ -166,4 +171,25 @@ Proof.
     + unfold apply_to in Hs'. exists s'. split. Lproc. intros v. split. 
       * intros m. specialize (H v) as [H1 H2]. rewrite H1. rewrite !eval_iff. rewrite <- !many_app_eq. now rewrite Hs'.
       * intros o. rewrite eval_iff. rewrite <- many_app_eq. rewrite Hs'. rewrite <- eval_iff. rewrite many_app_eq. eapply H.
+Qed.
+
+Lemma many_app_eq_nat {k} (v : Vector.t nat k) s :  many_app s (Vector.map enc v) = Vector.fold_left (fun (s : term) n => s (encNatL n)) s v.
+Proof.
+   induction v in s |- *.
+   * cbn. reflexivity.
+   * cbn. now rewrite IHv.
+Qed.
+
+Lemma L_computable_can_closed k R:
+  L_computable_closed R <-> L_computable (k:=k) R.
+Proof.
+  split.
+  - intros (s & _ & H). exists s. exact H.
+  - intros (s & H).
+    unshelve edestruct (@total_decodable_closed_new nat _ _ k s nat _  ) as (s' & Hcl & Hs'); try exact _.
+    + intros v o. rewrite <- eval_iff. intros. eapply (H v). unfold apply_to in H0. revert H0.
+      now rewrite many_app_eq_nat.
+    + unfold apply_to in Hs'. exists s'. split. Lproc. intros v. split. 
+      * intros m. specialize (H v) as [H1 H2]. rewrite H1. rewrite !eval_iff. rewrite <- !many_app_eq_nat. now rewrite Hs'.
+      * intros o. rewrite eval_iff. rewrite <- many_app_eq_nat. rewrite Hs'. rewrite <- eval_iff. rewrite many_app_eq_nat. eapply H.
 Qed.
