theories/TM/L/CompilerBoolFuns/LComp_to_TMComp.v
@@ -1,4 +1,4 @@
-From Undecidability.TM.L.CompilerBoolFuns Require Import Compiler_spec Compiler_facts Compiler ClosedLAdmissible.
+From Undecidability.TM.L.CompilerBoolFuns Require Import Compiler_spec Compiler_facts Compiler ClosedLAdmissible Compiler_nat_facts.
 
 Lemma L_bool_computable_to_TM_bool_computable k (R : Vector.t (list bool) k -> list bool -> Prop) :
   L_bool_computable R -> TM_bool_computable R.
@@ -10,4 +10,10 @@ Qed.
 
 Lemma L_computable_to_TM_computable k (R : Vector.t nat k -> nat -> Prop) :
   L_computable R -> TM_computable R.
-Admitted.
+Proof.
+  intros.
+  eapply TM_bool_computable_to_TM_computable.
+  eapply L_bool_computable_to_TM_bool_computable.
+  eapply L_computable_to_L_bool_computable.
+  eapply H.
+Qed.
